\begin{problem}
  (\textnormal{Problem~5.2.3}) Use the sample~${Y_1 = 8.2}$, ${Y_2 = 9.1}$, ${Y_3 = 10.6}$, and~${Y_4 = 4.9}$ to calculate the maximum likelihood estimate for~$\lambda$ in the exponential pdf:

  \begin{equation}\label{eq:P02:Exponential}
    f_{Y}(y;\lambda) = \lambda e^{-\lambda y}, \hspace{0.1cm} y \geq 0 \text{.}
  \end{equation}
\end{problem}

Given some i.i.d.\ sample~${Y_{1},\ldots,Y_{n}}$, the likelihood is

\begin{equation}\label{eq:P02:Likelihood}
  L_{n}(\lambda) = \lambda^{n}\exp\left(-\lambda\sum_{i=1}^{n} y_{i}\right)\text{.}
\end{equation}

\noindent
The log likelihood of the aforementioned sequence is

\begin{equation}\label{eq:P02:LogLikelihood}
  \ell(\lambda) = \ln\left(L(\lambda)\right) = n\ln(\lambda) - \lambda \sum_{i=1}^{n} y_i\text{.}
\end{equation}

\noindent
Its derivative is:

\begin{equation}\label{eq:P02:LogLikelihood:Derivative}
  \ell'(\lambda) = \frac{4}{\lambda} - \sum_{i=1}^{4} y_i = \frac{4}{\lambda} - 32.8  \text{.}
\end{equation}

\noindent
Setting the above equal to zero, we see that maximum likelihood estimate is

\begin{align}
  \frac{4}{\hat{\lambda}} - 32.8 &= 0 \\
  \hat{\lambda} &= \frac{4}{32.8} \\
                &\approx \boxed{0.1220} \text{.}
\end{align}
